deps/poulet4/lib/P4automata/Bisimulations.v
@@ -1,0 +1,571 @@
+Require Import Coq.micromega.Lia.
+Require Import Compare_dec.
+Require Import Coq.Lists.List.
+Require Import Coq.Classes.EquivDec.
+Import List.ListNotations.
+
+Require Import Poulet4.P4automata.P4automaton.
+Require Import Poulet4.FinType.
+Require Import Poulet4.P4automata.PreBisimulationSyntax.
+Require Import Poulet4.Relations.
+Require Poulet4.P4automata.WP.
+Require Poulet4.P4automata.WPSymBit.
+Require Poulet4.P4automata.WPSymLeap.
+Require Poulet4.P4automata.Reachability.
+
+Module SynPreSynWP.
+  Section SynPreSynWP.
+
+    (* State identifiers. *)
+    Variable (S1: Type).
+    Context `{S1_eq_dec: EquivDec.EqDec S1 eq}.
+    Context `{S1_finite: @Finite S1 _ S1_eq_dec}.
+
+    Variable (S2: Type).
+    Context `{S2_eq_dec: EquivDec.EqDec S2 eq}.
+    Context `{S2_finite: @Finite S2 _ S2_eq_dec}.
+
+    Definition S: Type := S1 + S2.
+
+    (* Header identifiers. *)
+    Variable (H: Type).
+    Context `{H_eq_dec: EquivDec.EqDec H eq}.
+    Context `{H_finite: @Finite H _ H_eq_dec}.
+
+    Variable (a: P4A.t S H).
+
+    Variable (wp: P4A.t S H ->
+                  conf_rel S H ->
+                  list (conf_rel S H)).
+
+    Notation conf := (configuration (P4A.interp a)).
+
+    Notation "⟦ x ⟧" := (interp_crel x).
+    Notation "⦇ x ⦈" := (interp_conf_rel (a:=a) x).
+    Notation "R ⊨ q1 q2" := (interp_crel R q1 q2) (at level 40).
+    Notation "R ⊨ S" := (forall q1 q2, ⟦R⟧ q1 q2 -> ⦇S⦈ q1 q2) (at level 40).
+    Notation δ := step.
+
+    Reserved Notation "R ⇝ S" (at level 10).
+    Inductive pre_bisimulation : crel S H -> crel S H -> relation conf :=
+    | PreBisimulationClose:
+        forall R q1 q2,
+          ⟦R⟧ q1 q2 ->
+          R ⇝ [] q1 q2
+    | PreBisimulationSkip:
+        forall (R T: crel S H) (C: conf_rel S H) q1 q2,
+          R ⊨ C ->
+          R ⇝ T q1 q2 ->
+          R ⇝ (C :: T) q1 q2
+    | PreBisimulationExtend:
+        forall (R T: crel S H) (C: conf_rel S H) q1 q2,
+          (C :: R) ⇝ (T ++ wp a C) q1 q2 ->
+          R ⇝ (C :: T) q1 q2
+    where "R ⇝ S" := (pre_bisimulation R S).
+
+    Fixpoint range (n: nat) :=
+      match n with
+      | 0 => []
+      | Datatypes.S n => range n ++ [n]
+      end.
+
+    Definition not_accept1 (a: P4A.t S H) (s: S) : crel S H := 
+      List.map (fun n =>
+                  {| cr_st := {| cs_st1 := {| st_state := inr true; st_buf_len := 0 |};
+                                 cs_st2 := {| st_state := inl s;    st_buf_len := n |} |};
+                     cr_rel := BRFalse _ BCEmp |})
+               (range (P4A.size a s)).
+
+    Definition not_accept2 (a: P4A.t S H) (s: S) : crel S H := 
+      List.map (fun n =>
+                  {| cr_st := {| cs_st1 := {| st_state := inl s;    st_buf_len := n |};
+                                 cs_st2 := {| st_state := inr true; st_buf_len := 0 |} |};
+                     cr_rel := BRFalse _ BCEmp |})
+               (range (P4A.size a s)).
+
+    Definition init_rel (a: P4A.t S H) : crel S H := 
+      List.concat (List.map (not_accept1 a) (enum S) ++
+                            List.map (not_accept2 a) (enum S)).
+    
+
+    Definition sum_not_accept1 (a: P4A.t (S1 + S2) H) (s: S1) : crel (S1 + S2) H := 
+      List.map (fun n =>
+                  {| cr_st := {| cs_st1 := {| st_state := inl (inl s); st_buf_len := n |};
+                                 cs_st2 := {| st_state := inr true;    st_buf_len := 0 |} |};
+                     cr_rel := BRFalse _ BCEmp |})
+               (range (P4A.size a (inl s))).
+
+    Definition sum_not_accept2 (a: P4A.t (S1 + S2) H) (s: S2) : crel (S1 + S2) H := 
+      List.map (fun n =>
+                  {| cr_st := {| cs_st1 := {| st_state := inr true;    st_buf_len := 0 |};
+                                 cs_st2 := {| st_state := inl (inr s); st_buf_len := n |} |};
+                     cr_rel := BRFalse _ BCEmp |})
+               (range (P4A.size a (inr s))).
+
+    Definition sum_init_rel (a: P4A.t (S1 + S2) H) : crel (S1 + S2) H := 
+      List.concat (List.map (sum_not_accept1 a) (enum S1)
+                            ++ List.map (sum_not_accept2 a) (enum S2)).
+    Notation "ctx , ⟨ s1 , n1 ⟩ ⟨ s2 , n2 ⟩ ⊢ b" :=
+      ({| cr_st :=
+            {| cs_st1 := {| st_state := s1; st_buf_len := n1 |};
+               cs_st2 := {| st_state := s2; st_buf_len := n2 |}; |};
+          cr_ctx := ctx;
+          cr_rel := b|}) (at level 10).
+    Notation btrue := (BRTrue _ _).
+    Notation bfalse := (BRFalse _ _).
+    Notation "a ⇒ b" := (BRImpl a b) (at level 40).
+
+    Definition reachable_pair_to_partition '((s1, s2): Reachability.state_pair _ _)
+      : crel (S1 + S2) H :=
+      match s1.(st_state) with
+      | inl st =>
+        [BCEmp, ⟨inl st, s1.(st_buf_len)⟩ ⟨inr true, 0⟩ ⊢ bfalse]
+      | inr st =>
+        []
+      end
+        ++
+        match s2.(st_state) with
+        | inl st =>
+          [BCEmp, ⟨inr true, 0⟩ ⟨inl st, s2.(st_buf_len)⟩ ⊢ bfalse]
+        | inr st =>
+          []
+        end.
+
+    Definition reachable_pairs_to_partition (r: Reachability.state_pairs _ _)
+      : crel (S1 + S2) H :=
+      List.concat (List.map reachable_pair_to_partition r).
+
+    Definition mk_init (n: nat) (a: P4A.t (S1 + S2) H) s1 s2 :=
+      let s := ({| st_state := inl (inl s1); st_buf_len := 0 |}, 
+                {| st_state := inl (inr s2); st_buf_len := 0 |}) in
+      List.nodup (@conf_rel_eq_dec _ _ _ _ _ _)
+                 (reachable_pairs_to_partition
+                    (Reachability.reachable_states a n [s])).
+  End SynPreSynWP.
+  Arguments pre_bisimulation {S1 S2 H equiv2 H_eq_dec} a wp.
+End SynPreSynWP.
+
+Module SemPre.
+  Section SemPre.
+    Variable (a: p4automaton).
+    Notation conf := (configuration a).
+
+    Notation "⟦ x ⟧" := (interp_rels x).
+    Notation "R ⊨ S" := (forall q1 q2,
+                            ⟦R⟧ q1 q2 ->
+                            S q1 q2)
+                          (at level 40).
+
+    Reserved Notation "R ⇝ S" (at level 10).
+    Inductive pre_bisimulation : rels conf -> rels conf -> rel conf :=
+    | PreBisimulationClose:
+        forall R q1 q2,
+          ⟦R⟧ q1 q2 ->
+          R ⇝ [] q1 q2
+    | PreBisimulationSkip:
+        forall R T (C: relation conf) q1 q2,
+          R ⊨ C ->
+          R ⇝ T q1 q2 ->
+          R ⇝ (C :: T) q1 q2
+    | PreBisimulationExtend:
+        forall R T C W q1 q2,
+          (C :: R) ⇝ (T ++ W) q1 q2 ->
+          (forall q1 q2, ⟦W⟧ q1 q2 -> (forall bit, C (step q1 bit) (step q2 bit))) ->
+          R ⇝ (C :: T) q1 q2
+    where "R ⇝ S" := (pre_bisimulation R S).
+
+  End SemPre.
+End SemPre.
+
+Module SemPreLeaps.
+  Section SemPreLeaps.
+    Variable (a: p4automaton).
+    Notation conf := (configuration a).
+
+    Notation "⟦ x ⟧" := (interp_rels x).
+    Notation "R ⊨ S" := (forall q1 q2,
+                            ⟦R⟧ q1 q2 ->
+                            S q1 q2)
+                          (at level 40).
+
+    Reserved Notation "R ⇝ S" (at level 10).
+    Inductive pre_bisimulation : rels conf -> rels conf -> rel conf :=
+    | PreBisimulationClose:
+        forall R q1 q2,
+          ⟦R⟧ q1 q2 ->
+          R ⇝ [] q1 q2
+    | PreBisimulationSkip:
+        forall R T (C: relation conf) q1 q2,
+          R ⊨ C ->
+          R ⇝ T q1 q2 ->
+          R ⇝ (C :: T) q1 q2
+    | PreBisimulationExtend:
+        forall R T C W q1 q2,
+          (C :: R) ⇝ (T ++ W) q1 q2 ->
+          (forall q1 q2, ⟦W⟧ q1 q2 -> (forall bit, C (step q1 bit) (step q2 bit))) ->
+          R ⇝ (C :: T) q1 q2
+    where "R ⇝ S" := (pre_bisimulation R S).
+
+  End SemPreLeaps.
+End SemPreLeaps.
+
+Module SemBisim.
+  Section SemBisim.
+    Variable (a: p4automaton).
+    Notation conf := (configuration a).
+
+    Definition bisimulation (R: rel conf) :=
+      forall q1 q2,
+        R q1 q2 ->
+        (accepting q1 <-> accepting q2) /\
+        forall b, R (step q1 b) (step q2 b).
+
+    Definition bisimilar q1 q2 :=
+      exists R, bisimulation R /\ R q1 q2.
+
+    Lemma bisimilar_implies_equiv :
+      forall (c1 c2: conf),
+        bisimilar c1 c2 ->
+        lang_equiv c1 c2.
+    Proof.
+      intros.
+      unfold lang_equiv.
+      intros; revert c1 c2 H.
+      induction input; intros.
+      - unfold accepted.
+        simpl.
+        unfold bisimilar in H.
+        destruct H as [R [? ?]].
+        now apply H in H0.
+      - unfold accepted.
+        repeat rewrite follow_cons.
+        apply IHinput.
+        unfold bisimilar in H.
+        destruct H as [R [? ?]].
+        exists R.
+        apply H in H0.
+        easy.
+    Qed.
+
+    Lemma lang_equiv_is_bisimulation :
+        bisimulation lang_equiv
+    .
+    Proof.
+      unfold bisimulation; intros.
+      split.
+      - apply (H nil).
+      - intros.
+        unfold lang_equiv.
+        intros.
+        unfold accepted.
+        repeat rewrite <- follow_cons.
+        apply H.
+    Qed.
+
+    Lemma equiv_implies_bisimilar
+          (c1 c2: conf)
+      :
+        lang_equiv c1 c2 -> bisimilar c1 c2
+    .
+    Proof.
+      intros.
+      exists lang_equiv.
+      split; try easy.
+      apply lang_equiv_is_bisimulation.
+    Qed.
+
+    Theorem bisimilar_iff_lang_equiv
+            (c1 c2: conf)
+      :
+        lang_equiv c1 c2 <-> bisimilar c1 c2
+    .
+    Proof.
+      split.
+      - apply equiv_implies_bisimilar.
+      - apply bisimilar_implies_equiv.
+    Qed.
+
+  End SemBisim.
+End SemBisim.
+
+Module SemBisimUpto.
+  Section SemBisimUpto.
+    Variable (a: p4automaton).
+    Notation conf := (configuration a).
+    Definition bisimulation_upto
+               (f: rel conf -> rel conf)
+               (R: rel conf)
+      :=
+        forall c1 c2,
+          R c1 c2 ->
+          (accepting c1 <-> accepting c2) /\
+          forall b, f R (step c1 b) (step c2 b)
+    .
+
+    Definition bisimilar_upto
+               (f: rel conf -> rel conf)
+               (c1 c2: conf)
+      :=
+        exists R, bisimulation_upto f R /\ R c1 c2
+    .
+
+    Definition closure_extends
+               (close: rel conf -> rel conf)
+      :=
+        forall (R: rel conf) c1 c2,
+          R c1 c2 -> close R c1 c2
+    .
+
+    Definition closure_preserves_accept
+               (close: rel conf -> rel conf)
+      :=
+        forall (R: rel conf),
+          (forall c1 c2, R c1 c2 -> accepting c1 <-> accepting c2) ->
+          (forall c1 c2, close R c1 c2 -> accepting c1 <-> accepting c2)
+    .
+
+    Definition closure_preserves_transition
+               (close: rel conf -> rel conf)
+      :=
+        forall (R: rel conf),
+          (forall c1 c2, R c1 c2 ->
+                    forall b, close R (step c1 b) (step c2 b)) ->
+          (forall c1 c2, close R c1 c2 ->
+                    forall b, close R (step c1 b) (step c2 b))
+    .
+
+    Definition closure_mono
+               (close: rel conf -> rel conf)
+      :=
+        forall (R R': rel conf),
+          (forall c1 c2, R c1 c2 -> R' c1 c2) ->
+          (forall c1 c2, close R c1 c2 -> close R' c1 c2)
+    .
+
+    Class SoundClosure
+          (f: rel conf -> rel conf)
+      := {
+      closure_sound_extends: closure_extends f;
+      closure_sound_preserves_accept: closure_preserves_accept f;
+      closure_sound_preserves_transition: closure_preserves_transition f;
+      closure_sound_mono: closure_mono f;
+        }.
+
+    Lemma bisimilar_implies_bisimilar_upto
+          (f: rel conf -> rel conf)
+      :
+        SoundClosure f ->
+        forall c1 c2,
+          SemBisim.bisimilar a c1 c2 ->
+          bisimilar_upto f c1 c2
+    .
+    Proof.
+      intros.
+      destruct H0 as [R [? ?]].
+      exists R; split; auto.
+      intros c1' c2' ?; split.
+      - now apply H0.
+      - intros.
+        now apply H, H0.
+    Qed.
+
+    Lemma bisimilar_upto_implies_bisimilar
+          (f: rel conf -> rel conf)
+      :
+        SoundClosure f ->
+        forall c1 c2,
+          bisimilar_upto f c1 c2 ->
+          SemBisim.bisimilar a c1 c2
+    .
+    Proof.
+      intros.
+      destruct H0 as [R [? ?]].
+      exists (f R); split.
+      - intros c1' c2' ?; split.
+        + revert c1' c2' H2.
+          now apply H, H0.
+        + revert c1' c2' H2.
+          now apply H, H0.
+      - now apply closure_sound_extends.
+    Qed.
+
+    (* Sanity check: the identity function is a valid closure. *)
+    Definition close_id (R: rel conf) := R.
+
+    Program Instance close_id_sound
+      : SoundClosure close_id
+    .
+    Solve Obligations with firstorder.
+
+  End SemBisimUpto.
+End SemBisimUpto.
+
+Module SemBisimLeaps.
+  Section SemBisimLeaps.
+    Variable (a: p4automaton).
+    Notation conf := (configuration a).
+
+    Inductive close_interpolate (R: rel conf) : rel conf :=
+      | InterpolateBase:
+          forall c1 c2,
+            R c1 c2 -> close_interpolate _ c1 c2
+      | InterpolateStep:
+          forall s1 st1 buf1 s2 st2 buf2 b,
+            close_interpolate R (inl s1, st1, buf1)
+                                (inl s2, st2, buf2) ->
+            length buf1 + 1 < size a s1 ->
+            length buf2 + 1 < size a s2 ->
+            (forall buf,
+                length buf = min (size a s1 - length buf1)
+                                 (size a s2 - length buf2) ->
+                R (follow (inl s1, st1, buf1) buf)
+                  (follow (inl s2, st2, buf2) buf)) ->
+            close_interpolate R (inl s1, st1, buf1 ++ b :: nil)
+                                (inl s2, st2, buf2 ++ b :: nil)
+    .
+
+    Program Instance close_interpolate_sound
+      : SemBisimUpto.SoundClosure a close_interpolate
+    .
+    Next Obligation.
+      eauto using InterpolateBase.
+    Qed.
+    Next Obligation.
+      induction H0; firstorder.
+    Qed.
+    Next Obligation.
+      revert b.
+      induction H0; intros; eauto.
+      repeat rewrite <- step_with_space; auto.
+      destruct (le_lt_dec (Nat.min (size a s1 - length buf1)
+                                   (size a s2 - length buf2)) 2).
+      - apply InterpolateBase.
+        rewrite <- follow_nil.
+        rewrite <- follow_nil at 1.
+        repeat rewrite <- follow_cons.
+        apply H3.
+        simpl length.
+        lia.
+      - repeat rewrite step_with_space;
+          repeat rewrite app_length;
+          simpl length;
+          try lia.
+        apply InterpolateStep;
+          repeat rewrite app_length;
+          simpl length;
+          try lia.
+        + repeat rewrite <- step_with_space; eauto.
+        + intros.
+          repeat rewrite <- follow_with_space; try lia.
+          apply H3.
+          simpl length.
+          lia.
+    Qed.
+    Next Obligation.
+      induction H0.
+      - eauto using InterpolateBase.
+      - eauto using InterpolateStep.
+    Qed.
+
+    Definition bisimulation_with_leaps
+               (R: rel conf)
+      :=
+        forall c1 c2,
+          R c1 c2 ->
+          (accepting c1 <-> accepting c2) /\
+          forall buf,
+            length buf = min (min_step c1) (min_step c2) ->
+            R (follow c1 buf) (follow c2 buf)
+    .
+
+    Definition bisimilar_with_leaps (c1 c2: conf) :=
+      exists R,
+        R c1 c2 /\ bisimulation_with_leaps R
+    .
+    
+    Lemma bisimilar_with_leaps_implies_bisimilar_upto
+          (c1 c2: conf)
+      :
+        bisimilar_with_leaps c1 c2 ->
+        SemBisimUpto.bisimilar_upto a close_interpolate c1 c2
+    .
+    Proof.
+      intros.
+      destruct H as [R [? ?]].
+      exists R.
+      split; auto.
+      intros c1' c2' ?; split.
+      - now apply H0.
+      - intros.
+        rewrite <- follow_nil.
+        rewrite <- follow_nil at 1.
+        repeat rewrite <- follow_cons.
+        destruct c1' as (([s1' | h1'], st1'), buf1'),
+                        c2' as (([s2' | h2'], st2'), buf2').
+        + destruct (Compare_dec.le_lt_dec 2 (min (min_step (inl s1', st1', buf1'))
+                                                 (min_step (inl s2', st2', buf2')))).
+          * repeat rewrite follow_with_space.
+            all: unfold min_step; simpl in l; try lia.
+            apply InterpolateStep; try lia.
+            now apply InterpolateBase.
+            intros.
+            apply H0; auto.
+            simpl min_step.
+            lia.
+          * apply InterpolateBase, H0; auto.
+            simpl min_step in *.
+            simpl length.
+            lia.
+        + apply InterpolateBase, H0; auto.
+          simpl min_step in *.
+          simpl length.
+          lia.
+        + apply InterpolateBase, H0; auto.
+          simpl min_step in *.
+          simpl length.
+          lia.
+        + apply InterpolateBase.
+          apply H0; auto.
+    Qed.
+
+    Lemma bisimilar_implies_bisimilar_with_leaps
+          (c1 c2: conf)
+      :
+        SemBisim.bisimilar a c1 c2 ->
+        bisimilar_with_leaps c1 c2
+    .
+    Proof.
+      intros.
+      destruct H as [R [? ?]].
+      exists R.
+      split; auto.
+      intros c1' c2' ?; split.
+      - now apply H.
+      - intros.
+        clear H2.
+        induction buf using rev_ind.
+        + now repeat rewrite follow_nil.
+        + unfold follow.
+          repeat rewrite fold_left_app.
+          fold (follow c1' buf).
+          fold (follow c2' buf).
+          simpl fold_left.
+          now apply H.
+    Qed.
+
+    Theorem bisimilar_iff_bisimilar_with_leaps
+            (c1 c2: conf)
+      :
+        SemBisim.bisimilar a c1 c2 <->
+        bisimilar_with_leaps c1 c2
+    .
+    Proof.
+      split; intro.
+      - now apply bisimilar_implies_bisimilar_with_leaps.
+      - apply SemBisimUpto.bisimilar_upto_implies_bisimilar with (f := close_interpolate).
+        + apply close_interpolate_sound.
+        + now apply bisimilar_with_leaps_implies_bisimilar_upto.
+    Qed.
+
+  End SemBisimLeaps.
+End SemBisimLeaps.
