deps/poulet4/lib/P4automata/Examples/BabyIPProofSmallInitLeap.v
@@ -1,0 +1,20 @@
+Require Import Poulet4.P4automata.Examples.ProofHeader.
+Require Import Poulet4.P4automata.Examples.BabyIP.
+
+(*
+Lemma prebisim_babyip:
+  pre_bisimulation BabyIP.aut
+                   (WPSymLeap.wp (H:=_))
+                   nil
+                   (mk_init 10 BabyIP.aut BabyIP1.Start BabyIP2.Start)
+                   (inl (inl BabyIP1.Start), [], [])
+                   (inl (inr BabyIP2.Start), [], []).
+Proof.
+  set (rel0 := mk_init 10 BabyIP.aut BabyIP1.Start BabyIP2.Start).
+  cbv in rel0.
+  subst rel0.
+  time (repeat (time solve_bisim')).
+  cbv in *.
+  intuition (try congruence).
+Time Qed.
+*)
