deps/poulet4/lib/P4automata/Examples/ProofHeader.v
@@ -1,0 +1,5 @@
+Require Export Poulet4.P4automata.PreBisimulationSyntax.
+Require Poulet4.P4automata.Bisimulations.
+Export Bisimulations.SynPreSynWP.
+Export List.ListNotations.
+Require Export Poulet4.P4automata.BisimChecker.
