deps/poulet4/lib/P4automata/Examples/SimpleSplitProofSmallInitLeap.v
@@ -1,0 +1,23 @@
+Require Import Poulet4.P4automata.Examples.ProofHeader.
+Require Import Poulet4.P4automata.Examples.SimpleSplit.
+
+Definition possibly_unsound_init_rel
+  : crel (Simple.state + Split.state) (Sum.H Simple.header Split.header)
+  :=
+    (mk_init 100 SimpleSplit.aut Simple.Start Split.StSplit1). 
+
+Lemma prebisim_simple_split_sym_small_init_leap:
+  pre_bisimulation SimpleSplit.aut
+                   (WPSymLeap.wp (H:=SimpleSplit.header))
+                   nil
+                   possibly_unsound_init_rel
+                   (inl (inl Simple.Start), [], [])
+                   (inl (inr Split.StSplit1), [], []).
+Proof.
+  set (r := possibly_unsound_init_rel).
+  cbv in r.
+  subst r.
+  time (repeat solve_bisim').
+  cbv in *.
+  intuition (try congruence).
+Qed.
