deps/poulet4/lib/Relations.v
@@ -1,0 +1,20 @@
+Require Export Coq.Relations.Relations.
+Require Export Coq.Classes.RelationClasses.
+Require Import Coq.Lists.List.
+Export ListNotations.
+
+Notation rel A := (relation A).
+Definition rels A :=
+  list (relation A).
+
+Definition rel_true: forall {A}, relation A :=
+  fun _ x y => True.
+
+Notation "⊤" := rel_true.
+Notation "x ⊓ y" := (relation_conjunction x y) (at level 40).
+
+Fixpoint interp_rels {A} (R: rels A) : relation A :=
+  match R with
+  | [] => ⊤
+  | r :: R' => r ⊓ interp_rels R'
+  end.
